src/datalog/FixpointSemantics.v
@@ -1,0 +1,64 @@
+(*usually, we work with proof-tree semantics.
+  here we prove them equivalent to some fixpoint semantics, which used to be used in the currently-broken QueryableToRunnable.v but are not currently used for anything.
+ *)
+
+  Definition F p Q Px :=
+    let '(P, x) := Px in
+    P x \/ Q (P, x) \/ exists hyps', Exists (fun r => rule_impl (one_step_derives p) r x hyps') p /\ Forall (fun x => Q (P, x)) hyps'.
+
+  Lemma F_mono p S1 S2 :
+    (forall x, S1 x -> S2 x) ->
+    (forall x, F p S1 x -> F p S2 x).
+  Proof.
+    cbv [F]. intros Hle [P x] H. intuition auto. fwd. right. right. eexists.
+    split; [eassumption|]. eapply Forall_impl; eauto. simpl. auto.
+  Qed.
+
+  Definition S_sane {U : Type} (S : (U -> Prop) * U -> Prop) :=
+    (forall P x, P x -> S (P, x)) /\
+      (forall P1 x P2,
+          S (P1, x) ->
+          (forall y, P1 y -> S (P2, y)) ->
+          S (P2, x)).
+
+  Lemma prog_impl_lfp p :
+    equiv (fun '(P, f) => prog_impl p P f) (lfp (F p)).
+  Proof.
+    cbv [equiv]. intros. cbv [prog_impl].
+    epose proof pftree_lfp as H. cbv [equiv] in H. rewrite H.
+    cbv [F]. reflexivity.
+  Qed.
+
+  Lemma S_sane_ext {U : Type} (P Q : (U -> Prop) * U -> Prop) :
+    equiv P Q ->
+    S_sane P ->
+    S_sane Q.
+  Proof.
+    cbv [equiv S_sane]. intros.
+    assert ((forall x, P x -> Q x) /\ (forall x, Q x -> P x)) by (split; intros; apply H; assumption).
+    fwd. eauto 9.
+  Qed.
+
+  Hint Unfold prog_impl : core.
+
+  Lemma S_sane_lfp p : S_sane (lfp (F p)).
+  Proof.
+    eapply S_sane_ext; [apply prog_impl_lfp|]. cbv [S_sane]. split; intros; eauto.
+    Fail Fail solve [induction H; eauto].
+    eapply pftree_trans. eapply pftree_weaken_hyp; eauto.
+  Qed.
+
+  (*this gets more complicated due to meta rules :((( *)
+  Lemma split_fixpoint (p : list rule) S :
+    (forall P x, P x -> S (P, x)) ->
+    (forall r, In r p -> fp (F [r]) S) <->
+      fp (F p) S.
+  Proof.
+    intros Sgood1. cbv [fp F]. split.
+    - intros H [P x] Hx. destruct Hx as [Hx| [Hx|Hx]]; eauto.
+      fwd. apply Exists_exists in Hxp0. fwd. eapply H; eauto 6. admit.
+    - intros H r Hr [P x] Hx. destruct Hx as [Hx| [Hx|Hx]]; eauto. fwd.
+      invert_list_stuff.
+      apply H. right. right. eexists. split; [|eassumption]. apply Exists_exists. eauto.
+      admit.
+  Abort.
